proof of positive case in loop, refactored main theorem and switch lemmas

src/C_strtoimax/Spec.v
@@ -42,7 +42,7 @@ Section Spec.
   Definition plus_char := (Int.repr 43).
   Definition zero_char := (Int.repr 48).
   
-  (* Representing negative and positive int *)
+  (* Representing negative and positive int using signedness *)
   Definition int_to_int64 (i : int) := Int64.repr (Int.signed i).
   
   Definition Sign s :=
@@ -50,6 +50,9 @@ Section Spec.
     | Signed => (Int.repr (-1))
     | Unsigned => Int.repr 1
     end.
+
+  Definition sign i :=
+    if (i == minus_char)%int then Signed else Unsigned.
   
   Definition mult_sign s value :=
     match s with
@@ -57,11 +60,12 @@ Section Spec.
     | Unsigned => value
     end.
   
-  Definition digit_to_num s i inp_value :=
+ (* Converting a single char into into a number given previous value *)   
+  Definition digit_to_num s i v :=
     match s with
-    | Signed => (Int64.neg inp_value * (Int64.repr 10) -
+    | Signed => (Int64.neg v * (Int64.repr 10) -
                  int_to_int64 (i - zero_char)%int)
-    | Unsigned => (inp_value * (Int64.repr 10) +
+    | Unsigned => (v * (Int64.repr 10) +
                    int_to_int64 (i - zero_char)%int)
     end.
       
@@ -69,31 +73,29 @@ Section Spec.
   Variable m : mem.
   Variable ge : genv.
   Variable e : env.
-  
+
+  (* Constants of the function *)
   Definition ASN1_INTMAX_MAX := (Int64.not 0) >> 1.
-  
-  Fact shift_pow2_div :
-    (Int64.shru (Int64.not Int64.zero) Int64.one) =
-    Int64.repr (Int64.max_unsigned / 2).
-  Proof.
-    replace (Int64.not Int64.zero) with (Int64.repr Int64.max_unsigned) by (auto with ints).
-    unfold Int64.shru.
-    f_equal.
-  Qed.
-  
   Definition upper_boundary := ASN1_INTMAX_MAX // (Int64.repr 10).
   Definition last_digit_max := ASN1_INTMAX_MAX % (Int64.repr 10).
   Definition last_digit_max_minus := (ASN1_INTMAX_MAX % (Int64.repr 10)) + 1.
+
+  Definition max_sign s :=
+    match s with
+    | Signed => last_digit_max_minus 
+    | Unsigned => last_digit_max
+    end.
   
   (* digits [0-9]*)
   Definition digits := map Int.repr [48;49;50;51;52;53;54;55;56;57].
   Definition is_digit (i : int) := existsb (fun j => Int.eq i j) digits.
-  (* Functional spec *)
   
+  (* Executable spec *)
+
+  (* Return type *)
   Record asn_strtoimax_lim_result :=
     { return_type : asn_strtox_result_e ;
       value : option int64 ;
-      intp : option addr ;
       memory : option mem ; 
       }.
   
@@ -103,7 +105,6 @@ Section Spec.
           | Some m' => 
             Some {| return_type := ASN_STRTOX_OK;
                     value := Some (mult_sign s value);
-                    intp := Some intp;                        
                     memory := Mem.storev Mint64 m' (vptr intp) (Vlong (mult_sign s value)) |}
           | None => None
           end        
@@ -115,48 +116,31 @@ Section Spec.
                    then asn_strtoimax_lim_loop (str++) fin intp
                         (value * (Int64.repr 10) + d) s last_digit n m
                    else if (value == upper_boundary) && (d <= last_digit)
-                        then match s with
-                               | Signed => asn_strtoimax_lim_loop (str++) fin intp
-                                   (digit_to_num Signed i value) Signed last_digit n m
-                               | Unsigned => asn_strtoimax_lim_loop (str++) fin intp
-                                   (digit_to_num Unsigned i value) Unsigned last_digit n m
-                             end
+                        then  asn_strtoimax_lim_loop (str++) fin intp
+                                   (digit_to_num s i value) s last_digit n m
                         else match (Mem.storev Mptr m'' (vptr fin) (vptr str)) with
                              | Some m' => 
                                Some {| return_type := ASN_STRTOX_ERROR_RANGE;
                                        value := None;
-                                       intp := None;                      
                                        memory := Some m' |}
                              | None => None
                              end                          
               else match (Mem.storev Mptr m'' (vptr fin) (vptr str)) with
                    | Some m' => Some {| return_type := ASN_STRTOX_EXTRA_DATA;
                                        value := Some (mult_sign s value);
-                                       intp := Some str;                      
                                        memory := Mem.storev Mint64 m' (vptr intp) (Vlong (mult_sign s value)) |}
                    | None => None
                    end
             | _ => None                
             end
     end.
-  
-  Definition sign i :=
-    if (i == minus_char)%int then Signed else Unsigned.
-  
-  (* Representing negative and positive int *)
-  Definition max_sign s :=
-    match s with
-    | Signed => last_digit_max_minus 
-    | Unsigned => last_digit_max
-    end.
-  
+
   Definition asn_strtoimax_lim (str fin intp : addr) : option asn_strtoimax_lim_result :=
     match load_addr Mptr m fin with (* derefencing **fin *)
     | Some (Vptr b ofs) =>
       match addr_ge m str (b, ofs) with (* compare str and *fin *)
       | Some true => Some {| return_type := ASN_STRTOX_ERROR_INVAL;
                                              value := None;
-                                             intp := None;                        
                                              memory := Some m; |}
       | Some false => let dist := distance str (b,ofs) in
                      match load_addr Mint8signed m str with
@@ -165,7 +149,6 @@ Section Spec.
                        then match addr_ge m (str++) (b,ofs) with
                             | Some true =>  Some {| return_type := ASN_STRTOX_EXPECT_MORE;
                                              value := None;
-                                             intp := None;                        
                                              memory := (Mem.storev Mptr m (vptr fin) (vptr (str++))); |}
   
                             | Some false => asn_strtoimax_lim_loop (str++) fin intp 0 (sign i) (max_sign (sign i)) (dist - 1)%nat m
@@ -178,5 +161,49 @@ Section Spec.
       end 
     | _ => None (* fail of pointer to fin *) 
     end.
+
+(* Abstract specification *)
+(* Z or int? *)
+Definition Z_of_ascii c := Z.of_nat (Ascii.nat_of_ascii c).
+
+Definition digit_to_Z s i v :=
+  match s with
+  | Signed => (-v* 10 - ((Z_of_ascii i) - 48))%Z
+  | Unsigned => (v * 10 - ((Z_of_ascii i) - 48))%Z
+  end.
+
+Definition long_of_ascii c := Int64.repr (Z.of_nat (Ascii.nat_of_ascii c)).
+Definition ascii_of_long i := Ascii.ascii_of_nat (Z.to_nat (Int64.unsigned i)).
+
+(* Let abstract string be a list of int *)
+Definition string_to_int (s : list int) (sign : signedness) :=
+  let
+    fix string_to_Z_loop (s : list int) (sign : signedness) (v : int64) :=
+      match s with
+      | nil => 0%Z
+      | char :: tl => string_to_Z_loop tl sign (digit_to_num sign char v)
+      end
+        in string_to_Z_loop s sign 0.
+    
+Definition addr_add (a : addr) (i : ptrofs) := match a with (b,ofs) => (b,(ofs+i)%ptrofs) end.
+
+Fixpoint string_at_address (s : list int) str dist : option (bool * list int) :=
+  match dist with
+  | O => Some (true, s)
+  | S n => match load_addr Mint8signed m str with
+          | Some (Vint i) => string_at_address (i::s) (str++) n
+          | _ => None
+          end
+  end.
+    
+Proposition asn_strtoimax_lim_fun_correct : forall s str fin intp m' val sign,
+    asn_strtoimax_lim str fin intp = Some {| return_type := ASN_STRTOX_OK ;
+                                             value := Some val ;
+                                             memory := m' |}
+                                       <->
+     addr_ge m str fin = Some false /\
+         string_at_address nil str (distance str fin) = Some (true,s) /\
+         string_to_int s sign = Int64.signed val.
+  Admitted.
 
 End Spec.
