src/C_strtoimax/Switch.v
@@ -7,80 +7,8 @@ Import ListNotations.
 Local Open Scope Int64Scope.
 
 (* Dealing with the switch statement *)
-Definition switch s1 s2 :=
-  (Sswitch (Ederef (Etempvar _str (tptr tschar)) tschar)
-    (LScons (Some 48)
-      Sskip
-      (LScons (Some 49)
-        Sskip
-        (LScons (Some 50)
-          Sskip
-          (LScons (Some 51) Sskip
-            (LScons (Some 52)
-              Sskip
-              (LScons (Some 53)
-                Sskip
-                (LScons (Some 54)
-                  Sskip
-                  (LScons (Some 55)
-                    Sskip
-                    (LScons (Some 56)
-                      Sskip
-                      (LScons (Some 57)
-                       s1 (LScons None
-                          s2
-                          LSnil)))))))))))).
 
-(* If reading i a digit then we enter the correct branch and continue *)
-Lemma switch_correct_continue : forall m ge e i s1 s2 le b ofs,
-    Mem.loadv Mint8signed m (Vptr b ofs) = Some (Vint i) ->
-    le ! _str = Some (Vptr b ofs) ->
-    is_digit i = true ->
-    forall le', (exists t, exec_stmt ge e le m s1 t le' m Out_continue) ->
-    (exists t, exec_stmt ge e le m (switch s1 s2) t le' m Out_continue).
-Proof.
-  intros.
-  cbn in H1.
-  break_exists.
-  repeat destruct_orb_hyp.
-  11: congruence.
-  all: assert (outcome_switch Out_continue = Out_continue) as Out by (simpl; auto); rewrite <- Out; repeat eexists; try reflexivity; repeat econstructor; try eassumption; try econstructor; (switch_destruct i).
-  1-9: eapply exec_Sseq_1; repeat (choose_seq s1); try (exec_Axiom || eassumption || discriminate).
-   eapply exec_Sseq_2. try (eassumption || econstructor || discriminate).
-   discriminate.
-Qed.
-
-(* If reading i a digit then we enter the correct branch and continue *)
-Lemma switch_default_correct : forall m ge e i s1 s2 le b ofs out,
-    Mem.loadv Mint8signed m (Vptr b ofs) = Some (Vint i) ->
-    le ! _str = Some (Vptr b ofs) ->
-    is_digit i = false ->
-    forall le' m', (exists t, exec_stmt ge e le m s2 t le' m' (Out_return out)) ->
-                (exists t, exec_stmt ge e le m (switch s1 s2) t le' m' (Out_return out)).
-Proof.
-  intros until out; intros Mem Str Dig le' m' S2.
-  destruct S2 as [t S2].
-  repeat eexists.
-  replace (Out_return out) with (outcome_switch (Out_return out)) by (reflexivity).
-  econstructor.
-  repeat econstructor; try eassumption.
-  econstructor.
-  cbn in Dig.
-  repeat destruct_orb_hyp.
-  repeat (switch_destruct i).
-  try (rewrite Int.unsigned_repr in *).
-  unfold select_switch.
-  unfold select_switch_default.
-  unfold select_switch_case.
-  repeat break_if.
-  all: try congruence.
-  eapply exec_Sseq_2.
-  eassumption.
-  discriminate.
-  all: cbn;  try lia.
-Qed.
-
-Definition switch_1 := (Sswitch (Ederef (Etempvar _str (tptr tschar)) tschar)
+Definition switch := (Sswitch (Ederef (Etempvar _str (tptr tschar)) tschar)
               (LScons (Some 45)
                 (Ssequence
                   (Sset _last_digit_max
@@ -107,12 +35,12 @@ Definition switch_1 := (Sswitch (Ederef (Etempvar _str (tptr tschar)) tschar)
                         Sskip)))
                   LSnil))).
 
-Lemma switch_default_correct_1 : forall m ge e i le b ofs,
+Lemma switch_default_correct : forall m ge e i le b ofs,
     Mem.loadv Mint8signed m (Vptr b ofs) = Some (Vint i) ->
     le ! _str = Some (Vptr b ofs) ->
     (i == minus_char)%int = false ->
     (i == plus_char)%int = false ->
-                (exists t, exec_stmt ge e le m switch_1 t le m Out_normal).
+                (exists t, exec_stmt ge e le m switch t le m Out_normal).
 Proof.
   unfold plus_char, minus_char.
   intros until ofs; intros Mem Str Min Plus.
@@ -131,24 +59,6 @@ Proof.
   econstructor.
   all: cbn;  try lia.
 Qed.     
-
-Lemma switch_correct_return : forall m ge e i s1 s2 le b ofs out,
-    Mem.loadv Mint8signed m (Vptr b ofs) = Some (Vint i) ->
-    le ! _str = Some (Vptr b ofs) ->
-    is_digit i = true ->
-    forall le' m', (exists t, exec_stmt ge e le m s1 t le' m' (Out_return out)) ->
-    (exists t, exec_stmt ge e le m (switch s1 s2) t le' m' (Out_return out)).
-Proof.
-  intros.
-  cbn in H1.
-  break_exists.
-  repeat destruct_orb_hyp.
-  11: congruence.
-  all: assert (outcome_switch (Out_return out) = (Out_return out)) as Out by (simpl; auto); rewrite <- Out; repeat eexists; try reflexivity; repeat econstructor; try eassumption; try econstructor; (switch_destruct i).
-  1-9: eapply exec_Sseq_1; repeat (choose_seq s1); try (exec_Axiom || eassumption || discriminate).
-   eapply exec_Sseq_2. try (eassumption || econstructor || discriminate).
-   discriminate.
-Qed.
 
 Lemma exec_loop_minus : forall m ge e le b ofs str_b str_ofs fin_b fin_ofs intp_b intp_ofs i out s1 s2,
     le!_str = Some (Vptr str_b str_ofs)  ->
@@ -178,58 +88,6 @@ Lemma exec_loop_minus : forall m ge e le b ofs str_b str_ofs fin_b fin_ofs intp_
                               m s1 t le' m' (Out_return out)) ->
         exists t le', exec_stmt ge e le m (pre_loop s1 s2) t le' m' (Out_return out).
 Proof.
-  intros until s2.
-  intros Str End Intp UB Sign LA AG LA' Char m' S1.
-  break_exists.
-  unfold pre_loop.
-  repeat eexists.
-  econstructor.
-  repeat econstructor.
-  econstructor.
-  repeat econstructor.
-  econstructor.
-  repeat econstructor.
-  econstructor.
-  repeat econstructor.
-  Tactics.forward.
-  unfold load_addr in *.
-  eassumption.
-  repeat env_assumption.
-  env_assumption.
-  econstructor.
-  repeat econstructor.
- assert (sem_binary_operation ge Oge (Vptr str_b str_ofs) (typeof (Etempvar _str (tptr tschar)))
-                              (Vptr b ofs) (typeof (Etempvar _t'6 (tptr tschar))) m = Some Vfalse)  by admit; eassumption.
- Tactics.forward.
- econstructor.
- econstructor.
- repeat econstructor.
- repeat env_assumption.
- eassumption.
- replace Out_normal with (outcome_switch Out_normal).
- econstructor.
- repeat econstructor.
- repeat env_assumption.
- eassumption.
- econstructor.
- replace i with (minus_char) by admit.
- econstructor.
- repeat econstructor.
- repeat env_assumption.
- econstructor.
- repeat econstructor.
- Tactics.forward.
- simpl.
- assert (sem_cmp Cge (Vptr str_b (str_ofs + Ptrofs.repr 1 * Ptrofs.of_ints (Int.repr 1))%ptrofs)
-                 (tptr tschar) (Vptr b ofs) (tptr tschar) m = Some Vfalse) by admit; eassumption.
- Tactics.forward.
- econstructor.
- reflexivity.
- apply exec_Sseq_2.
- econstructor.
- repeat econstructor.
- eapply H.
- discriminate.
 Admitted.
 
 Lemma exec_loop_plus : forall m ge e le b ofs str_b str_ofs fin_b fin_ofs intp_b intp_ofs i out s1 s2,
@@ -265,65 +123,6 @@ Lemma exec_loop_plus : forall m ge e le b ofs str_b str_ofs fin_b fin_ofs intp_b
                                                    ((_sign <~ Vint (Int.repr 1)) le)))))))*)
                               m s1 t le' m' (Out_return out)) ->
           exists t le', exec_stmt ge e le m (pre_loop s1 s2) t le' m' (Out_return out).
-Proof.
-  intros until s2.
-  intros Str End Intp UB Sign LA AG LA' Char m' S1.
-  break_exists.
-  unfold pre_loop.
-  repeat eexists.
-  econstructor.
-  repeat econstructor.
-  econstructor.
-  repeat econstructor.
-  econstructor.
-  repeat econstructor.
-  econstructor.
-  repeat econstructor.
-  Tactics.forward.
-  unfold load_addr in *.
-  eassumption.
-  repeat env_assumption.
-  env_assumption.
-  econstructor.
-  repeat econstructor.
-  assert (sem_binary_operation ge Oge (Vptr str_b str_ofs) (typeof (Etempvar _str (tptr tschar)))
-                               (Vptr b ofs) (typeof (Etempvar _t'6 (tptr tschar))) m = Some Vfalse) by admit; eassumption.
-  Tactics.forward.
-  econstructor.
-  econstructor.
-  repeat econstructor.
-  repeat env_assumption.
-  eassumption.
-  replace Out_normal with (outcome_switch Out_normal).
-  econstructor.
-  repeat econstructor.
-  repeat env_assumption.
-  eassumption.
-  econstructor.
-  replace i with (plus_char) by admit.
-  econstructor.
-  repeat econstructor.
-  repeat env_assumption.
-  econstructor.
-  repeat econstructor.
-  Tactics.forward.
-  simpl.
-  assert (sem_cmp Cge (Vptr str_b (str_ofs + Ptrofs.repr 1 * Ptrofs.of_ints (Int.repr 1))%ptrofs)
-                  (tptr tschar) (Vptr b ofs) (tptr tschar) m = Some Vfalse) by admit; eassumption.
-  Tactics.forward.
-  Tactics.forward.
-  simpl.
-  assert (sem_cmp Cge (Vptr str_b (str_ofs + Ptrofs.repr 1 * Ptrofs.of_ints (Int.repr 1))%ptrofs)
-                  (tptr tschar) (Vptr b ofs) (tptr tschar) m = Some Vfalse) by admit; eassumption.
-  repeat econstructor.
-  econstructor.
-  econstructor.
-  reflexivity.
-  apply exec_Sseq_2.
-  econstructor.
-  repeat econstructor.
-  eapply H.
-  discriminate.
 Admitted.
 
 Lemma exec_loop_none : forall m ge e le b ofs str_b str_ofs fin_b fin_ofs intp_b intp_ofs i out s1 s2,
@@ -357,64 +156,4 @@ Lemma exec_loop_none : forall m ge e le b ofs str_b str_ofs fin_b fin_ofs intp_b
                               m s1 t le' m' (Out_return out)) ->
                    
           exists t le', exec_stmt ge e le m (pre_loop s1 s2) t le' m' (Out_return out).
-Proof.
-  intros until s2.
-  intros Str End Intp UB Sign LA AG LA' CharP CharM  m' S1.
-  destruct S1.
-  unfold pre_loop.
-  destruct (switch_default_correct_1 m ge e i (in le set [
-                                                  _t'4 <~ Vint i ;
-                                                  _t'6 <~ Vptr b ofs ;
-                                                  _last_digit_max <~ Vlong
-                                                                  (Int64.modu
-                                                                     (Int64.not (cast_int_long Signed (Int.repr 0)) >>
-                                                                              Int64.repr (Int.unsigned (Int.repr 1)))
-                                                                     (cast_int_long Signed (Int.repr 10))) ;
-                                                  _upper_boundary <~ Vlong
-                                                                  (Int64.divu
-                                                                     (Int64.not (cast_int_long Signed (Int.repr 0)) >>
-                                                                              Int64.repr (Int.unsigned (Int.repr 1))) 
-                                                                     (cast_int_long Signed (Int.repr 10))) ;
-                                                  _sign <~ Vint (Int.repr 1)])
-                                     str_b str_ofs).
-  all: try eassumption; env_assumption.
-  repeat rewrite set_env_eq_ptree_set.
-  
-  repeat env_assumption.
-  repeat rewrite set_env_eq_ptree_set in H.
-  destruct H.
-  repeat eexists.
-  econstructor.
-  repeat econstructor.
-  econstructor.
-  repeat econstructor.
-  econstructor.
-  repeat econstructor.
-  econstructor.
-  repeat econstructor.
-  Tactics.forward.
-  unfold load_addr in *.
-  eassumption.
-  repeat env_assumption.
-  env_assumption.
-  econstructor.
-  repeat econstructor.
-  assert (sem_binary_operation ge Oge (Vptr str_b str_ofs) (typeof (Etempvar _str (tptr tschar)))
-                               (Vptr b ofs) (typeof (Etempvar _t'6 (tptr tschar))) m = Some Vfalse)
-    by admit;
-    eassumption.
-  Tactics.forward.
-  econstructor.
-  econstructor.
-  econstructor.
-  repeat econstructor.
-  repeat env_assumption.
-  eassumption.
-  (* something breakes here after I added notation
-  eassumption.
-  apply exec_Sseq_2.
-  econstructor.
-  repeat econstructor.
-  eassumption.
-  congruence.*)
 Admitted.
