src/C_strtoimax/AST.v
@@ -3,129 +3,158 @@ Require Export Clight.INTEGER.
 
 Definition f_asn_strtoimax_lim_loop :=
   (Sloop
-    (Ssequence
-      (Ssequence
-        (Sset _t'3
-          (Ederef (Etempvar _end (tptr (tptr tschar)))
-            (tptr tschar)))
-        (Sifthenelse (Ebinop Olt (Etempvar _str (tptr tschar))
-                       (Etempvar _t'3 (tptr tschar)) tint)
-          Sskip
-          Sbreak))
-      (Ssequence
-        (Sset _t'1 (Ederef (Etempvar _str (tptr tschar)) tschar))
-        (Sswitch (Ederef (Etempvar _str (tptr tschar)) tschar)
-          (LScons (Some 48)
-            Sskip
-            (LScons (Some 49)
-              Sskip
-              (LScons (Some 50)
-                Sskip
-                (LScons (Some 51)
-                  Sskip
-                  (LScons (Some 52)
-                    Sskip
-                    (LScons (Some 53)
-                      Sskip
-                      (LScons (Some 54)
+                  (Ssequence
+                    (Ssequence
+                      (Sset _t'9
+                        (Ederef (Etempvar _end (tptr (tptr tschar)))
+                          (tptr tschar)))
+                      (Sifthenelse (Ebinop Olt (Etempvar _str (tptr tschar))
+                                     (Etempvar _t'9 (tptr tschar)) tint)
                         Sskip
-                        (LScons (Some 55)
-                          Sskip
-                          (LScons (Some 56)
-                            Sskip
-                            (LScons (Some 57)
-                              (Ssequence
+                        Sbreak))
+                    (Ssequence
+                      (Ssequence
+                        (Sset _t'7
+                          (Ederef (Etempvar _str (tptr tschar)) tschar))
+                        (Sifthenelse (Ebinop Oge (Etempvar _t'7 tschar)
+                                       (Econst_int (Int.repr 48) tint) tint)
+                          (Ssequence
+                            (Sset _t'8
+                              (Ederef (Etempvar _str (tptr tschar)) tschar))
+                            (Sset _t'2
+                              (Ecast
+                                (Ebinop Ole (Etempvar _t'8 tschar)
+                                  (Econst_int (Int.repr 57) tint) tint)
+                                tbool)))
+                          (Sset _t'2 (Econst_int (Int.repr 0) tint))))
+                      (Sifthenelse (Etempvar _t'2 tint)
+                        (Ssequence
+                          (Ssequence
+                            (Sset _t'6
+                              (Ederef (Etempvar _str (tptr tschar)) tschar))
+                            (Sset _d
+                              (Ebinop Osub (Etempvar _t'6 tschar)
+                                (Econst_int (Int.repr 48) tint) tint)))
+                          (Sifthenelse (Ebinop Olt (Etempvar _value tlong)
+                                         (Etempvar _upper_boundary tlong)
+                                         tint)
+                            (Sset _value
+                              (Ebinop Oadd
+                                (Ebinop Omul (Etempvar _value tlong)
+                                  (Econst_int (Int.repr 10) tint) tlong)
+                                (Etempvar _d tint) tlong))
+                            (Sifthenelse (Ebinop Oeq (Etempvar _value tlong)
+                                           (Etempvar _upper_boundary tlong)
+                                           tint)
+                              (Sifthenelse (Ebinop Ole (Etempvar _d tint)
+                                             (Etempvar _last_digit_max tlong)
+                                             tint)
                                 (Ssequence
-                                  (Sset _t'2
-                                    (Ederef
-                                      (Etempvar _str (tptr tschar))
-                                      tschar))
-                                  (Sset _d
-                                    (Ebinop Osub
-                                      (Etempvar _t'2 tschar)
-                                      (Econst_int (Int.repr 48) tint)
-                                      tint)))
-                                (Ssequence
-                                  (Sifthenelse (Ebinop Olt
-                                                 (Etempvar _value tlong)
-                                                 (Etempvar _upper_boundary tlong)
+                                  (Sifthenelse (Ebinop Ogt
+                                                 (Etempvar _sign tint)
+                                                 (Econst_int (Int.repr 0) tint)
                                                  tint)
                                     (Sset _value
                                       (Ebinop Oadd
-                                        (Ebinop Omul
-                                          (Etempvar _value tlong)
+                                        (Ebinop Omul (Etempvar _value tlong)
                                           (Econst_int (Int.repr 10) tint)
-                                          tlong)
-                                        (Etempvar _d tint) tlong))
-                                    (Sifthenelse (Ebinop Oeq
-                                                   (Etempvar _value tlong)
-                                                   (Etempvar _upper_boundary tlong)
-                                                   tint)
-                                      (Sifthenelse (Ebinop Ole
-                                                     (Etempvar _d tint)
-                                                     (Etempvar _last_digit_max tlong)
-                                                     tint)
-                                        (Sifthenelse (Ebinop Ogt
-                                                       (Etempvar _sign tint)
-                                                       (Econst_int (Int.repr 0) tint)
-                                                       tint)
-                                          (Sset _value
-                                            (Ebinop Oadd
-                                              (Ebinop Omul
-                                                (Etempvar _value tlong)
-                                                (Econst_int (Int.repr 10) tint)
-                                                tlong)
-                                              (Etempvar _d tint)
-                                              tlong))
-                                          (Ssequence
-                                            (Sset _sign
-                                              (Econst_int (Int.repr 1) tint))
-                                            (Sset _value
-                                              (Ebinop Osub
-                                                (Ebinop Omul
-                                                  (Eunop Oneg
-                                                    (Etempvar _value tlong)
-                                                    tlong)
-                                                  (Econst_int (Int.repr 10) tint)
-                                                  tlong)
-                                                (Etempvar _d tint)
-                                                tlong))))
-                                        (Ssequence
-                                          (Sassign
-                                            (Ederef
-                                              (Etempvar _end (tptr (tptr tschar)))
-                                              (tptr tschar))
-                                            (Etempvar _str (tptr tschar)))
-                                          (Sreturn (Some (Econst_int (Int.repr (-3)) tint)))))
+                                          tlong) (Etempvar _d tint) tlong))
+                                    (Ssequence
+                                      (Sset _sign
+                                        (Econst_int (Int.repr 1) tint))
+                                      (Sset _value
+                                        (Ebinop Osub
+                                          (Ebinop Omul
+                                            (Eunop Oneg
+                                              (Etempvar _value tlong) tlong)
+                                            (Econst_int (Int.repr 10) tint)
+                                            tlong) (Etempvar _d tint) tlong))))
+                                  (Ssequence
+                                    (Sset _str
+                                      (Ebinop Oadd
+                                        (Etempvar _str (tptr tschar))
+                                        (Econst_int (Int.repr 1) tint)
+                                        (tptr tschar)))
+                                    (Ssequence
                                       (Ssequence
-                                        (Sassign
+                                        (Sset _t'3
                                           (Ederef
                                             (Etempvar _end (tptr (tptr tschar)))
-                                            (tptr tschar))
-                                          (Etempvar _str (tptr tschar)))
-                                        (Sreturn (Some (Econst_int (Int.repr (-3)) tint))))))
-                                  Scontinue))
-                              (LScons None
+                                            (tptr tschar)))
+                                        (Sifthenelse (Ebinop Olt
+                                                       (Etempvar _str (tptr tschar))
+                                                       (Etempvar _t'3 (tptr tschar))
+                                                       tint)
+                                          (Ssequence
+                                            (Sassign
+                                              (Ederef
+                                                (Etempvar _end (tptr (tptr tschar)))
+                                                (tptr tschar))
+                                              (Etempvar _str (tptr tschar)))
+                                            (Ssequence
+                                              (Ssequence
+                                                (Sset _t'4
+                                                  (Ederef
+                                                    (Etempvar _str (tptr tschar))
+                                                    tschar))
+                                                (Sifthenelse (Ebinop Oge
+                                                               (Etempvar _t'4 tschar)
+                                                               (Econst_int (Int.repr 48) tint)
+                                                               tint)
+                                                  (Ssequence
+                                                    (Sset _t'5
+                                                      (Ederef
+                                                        (Etempvar _str (tptr tschar))
+                                                        tschar))
+                                                    (Sset _t'1
+                                                      (Ecast
+                                                        (Ebinop Ole
+                                                          (Etempvar _t'5 tschar)
+                                                          (Econst_int (Int.repr 57) tint)
+                                                          tint) tbool)))
+                                                  (Sset _t'1
+                                                    (Econst_int (Int.repr 0) tint))))
+                                              (Sifthenelse (Etempvar _t'1 tint)
+                                                (Sreturn (Some (Econst_int (Int.repr (-3)) tint)))
+                                                (Ssequence
+                                                  (Sassign
+                                                    (Ederef
+                                                      (Etempvar _intp (tptr tlong))
+                                                      tlong)
+                                                    (Ebinop Omul
+                                                      (Etempvar _sign tint)
+                                                      (Etempvar _value tlong)
+                                                      tlong))
+                                                  (Sreturn (Some (Econst_int (Int.repr 1) tint)))))))
+                                          Sskip))
+                                      Sbreak)))
                                 (Ssequence
                                   (Sassign
                                     (Ederef
                                       (Etempvar _end (tptr (tptr tschar)))
                                       (tptr tschar))
                                     (Etempvar _str (tptr tschar)))
-                                  (Ssequence
-                                    (Sassign
-                                      (Ederef
-                                        (Etempvar _intp (tptr tlong))
-                                        tlong)
-                                      (Ebinop Omul
-                                        (Etempvar _sign tint)
-                                        (Etempvar _value tlong)
-                                        tlong))
-                                    (Sreturn (Some (Econst_int (Int.repr 1) tint)))))
-                                LSnil))))))))))))))
-    (Sset _str
-      (Ebinop Oadd (Etempvar _str (tptr tschar))
-              (Econst_int (Int.repr 1) tint) (tptr tschar)))).
+                                  (Sreturn (Some (Econst_int (Int.repr (-3)) tint)))))
+                              (Ssequence
+                                (Sassign
+                                  (Ederef
+                                    (Etempvar _end (tptr (tptr tschar)))
+                                    (tptr tschar))
+                                  (Etempvar _str (tptr tschar)))
+                                (Sreturn (Some (Econst_int (Int.repr (-3)) tint)))))))
+                        (Ssequence
+                          (Sassign
+                            (Ederef (Etempvar _end (tptr (tptr tschar)))
+                              (tptr tschar)) (Etempvar _str (tptr tschar)))
+                          (Ssequence
+                            (Sassign
+                              (Ederef (Etempvar _intp (tptr tlong)) tlong)
+                              (Ebinop Omul (Etempvar _sign tint)
+                                (Etempvar _value tlong) tlong))
+                            (Sreturn (Some (Econst_int (Int.repr 1) tint))))))))
+                  (Sset _str
+                    (Ebinop Oadd (Etempvar _str (tptr tschar))
+                      (Econst_int (Int.repr 1) tint) (tptr tschar)))).
 
 
 Notation set_vars_switch_body :=
@@ -294,58 +323,58 @@ Notation switch_default :=
 Definition pre_loop s2 s3 := (Ssequence
   (Sset _sign (Econst_int (Int.repr 1) tint))
   (Ssequence
-    (Sset _upper_boundary
-      (Ebinop Odiv
-        (Ebinop Oshr
-          (Eunop Onotint (Ecast (Econst_int (Int.repr 0) tint) tulong)
-            tulong) (Econst_int (Int.repr 1) tint) tulong)
-        (Econst_int (Int.repr 10) tint) tulong))
+    (Sset _asn1_intmax_max
+      (Ebinop Oshr
+        (Eunop Onotint (Ecast (Econst_int (Int.repr 0) tint) tulong) tulong)
+        (Econst_int (Int.repr 1) tint) tulong))
     (Ssequence
-      (Sset _last_digit_max
-        (Ebinop Omod
-          (Ebinop Oshr
-            (Eunop Onotint (Ecast (Econst_int (Int.repr 0) tint) tulong)
-              tulong) (Econst_int (Int.repr 1) tint) tulong)
-          (Econst_int (Int.repr 10) tint) tulong))
+      (Sset _upper_boundary
+        (Ebinop Odiv (Etempvar _asn1_intmax_max tlong)
+          (Econst_int (Int.repr 10) tint) tlong))
       (Ssequence
-        (Ssequence
-          (Sset _t'6
-            (Ederef (Etempvar _end (tptr (tptr tschar))) (tptr tschar)))
-          (Sifthenelse (Ebinop Oge (Etempvar _str (tptr tschar))
-                         (Etempvar _t'6 (tptr tschar)) tint)
-            (Sreturn (Some (Econst_int (Int.repr (-2)) tint)))
-            Sskip))
+        (Sset _last_digit_max
+          (Ebinop Omod (Etempvar _asn1_intmax_max tlong)
+            (Econst_int (Int.repr 10) tint) tlong))
         (Ssequence
           (Ssequence
-            (Sset _t'4 (Ederef (Etempvar _str (tptr tschar)) tschar))
-            (Sswitch (Ederef (Etempvar _str (tptr tschar)) tschar)
-              (LScons (Some 45)
-                (Ssequence
-                  (Sset _last_digit_max
-                    (Ebinop Oadd (Etempvar _last_digit_max tlong)
-                      (Econst_int (Int.repr 1) tint) tlong))
-                  (Sset _sign
-                    (Eunop Oneg (Econst_int (Int.repr 1) tint) tint)))
-                (LScons (Some 43)
-                  (Ssequence
-                    (Sset _str
-                      (Ebinop Oadd (Etempvar _str (tptr tschar))
-                        (Econst_int (Int.repr 1) tint) (tptr tschar)))
-                    (Ssequence
-                      (Sset _t'5
-                        (Ederef (Etempvar _end (tptr (tptr tschar)))
-                          (tptr tschar)))
-                      (Sifthenelse (Ebinop Oge (Etempvar _str (tptr tschar))
-                                     (Etempvar _t'5 (tptr tschar)) tint)
-                        (Ssequence
-                          (Sassign
-                            (Ederef (Etempvar _end (tptr (tptr tschar)))
-                              (tptr tschar)) (Etempvar _str (tptr tschar)))
-                          (Sreturn (Some (Econst_int (Int.repr (-1)) tint))))
-                        Sskip)))
-                  LSnil))))
+            (Sset _t'12
+              (Ederef (Etempvar _end (tptr (tptr tschar))) (tptr tschar)))
+            (Sifthenelse (Ebinop Oge (Etempvar _str (tptr tschar))
+                           (Etempvar _t'12 (tptr tschar)) tint)
+              (Sreturn (Some (Econst_int (Int.repr (-2)) tint)))
+              Sskip))
           (Ssequence
             (Ssequence
-               (Sset _value (Ecast (Econst_int (Int.repr 0) tint) tlong))
+              (Sset _t'10 (Ederef (Etempvar _str (tptr tschar)) tschar))
+              (Sswitch (Ederef (Etempvar _str (tptr tschar)) tschar)
+                (LScons (Some 45)
+                  (Ssequence
+                    (Sset _last_digit_max
+                      (Ebinop Oadd (Etempvar _last_digit_max tlong)
+                        (Econst_int (Int.repr 1) tint) tlong))
+                    (Sset _sign
+                      (Eunop Oneg (Econst_int (Int.repr 1) tint) tint)))
+                  (LScons (Some 43)
+                    (Ssequence
+                      (Sset _str
+                        (Ebinop Oadd (Etempvar _str (tptr tschar))
+                          (Econst_int (Int.repr 1) tint) (tptr tschar)))
+                      (Ssequence
+                        (Sset _t'11
+                          (Ederef (Etempvar _end (tptr (tptr tschar)))
+                            (tptr tschar)))
+                        (Sifthenelse (Ebinop Oge
+                                       (Etempvar _str (tptr tschar))
+                                       (Etempvar _t'11 (tptr tschar)) tint)
+                          (Ssequence
+                            (Sassign
+                              (Ederef (Etempvar _end (tptr (tptr tschar)))
+                                (tptr tschar)) (Etempvar _str (tptr tschar)))
+                            (Sreturn (Some (Econst_int (Int.repr (-1)) tint))))
+                          Sskip)))
+                    LSnil))))
+            (Ssequence
+              (Ssequence
+                (Sset _value (Ecast (Econst_int (Int.repr 0) tint) tlong))
                s2)
-            s3)))))).
+            s3))))))).
